refactor statements and execution

HolBASimps.sml
@@ -26,11 +26,12 @@ val bir_list_of_types = [
    mk_thy_type {Tyop="bir_env_cond_t",       Thy="bir_env", Args=[]},
 
    mk_thy_type {Tyop="bir_label_t",          Thy="bir_program", Args=[]},
+   mk_thy_type {Tyop="bir_stmt_end_t",       Thy="bir_program", Args=[]},
+   mk_thy_type {Tyop="bir_stmt_basic_t",     Thy="bir_program", Args=[]},
    mk_thy_type {Tyop="bir_stmt_t",           Thy="bir_program", Args=[]},
    mk_thy_type {Tyop="bir_block_t",          Thy="bir_program", Args=[]},
    mk_thy_type {Tyop="bir_program_t",        Thy="bir_program", Args=[]},
    mk_thy_type {Tyop="bir_programcounter_t", Thy="bir_program", Args=[]},
-   mk_thy_type {Tyop="bir_status_finished_t",Thy="bir_program", Args=[]},
    mk_thy_type {Tyop="bir_status_t",         Thy="bir_program", Args=[]},
    mk_thy_type {Tyop="bir_state_t",          Thy="bir_program", Args=[]}
 ];
