bir_programScript.sml
@@ -17,31 +17,41 @@ val _ = Datatype `bir_label_t =
   | BL_Address bir_imm_t
 `;
 
-val _ = Datatype `bir_stmt_t =
+
+val _ = Datatype `bir_stmt_basic_t =
   | BStmt_Declare bir_var_t
   | BStmt_Assign  bir_var_t bir_exp_t
-  | BStmt_Jmp     bir_label_t
-  | BStmt_CJmp    bir_exp_t bir_label_t bir_label_t
-  | BStmt_Halt    bir_exp_t
   | BStmt_Assert  bir_exp_t
   | BStmt_Assume  bir_exp_t
 `;
 
-val _ = Datatype `bir_block_t = <| bb_label:bir_label_t ; bb_statements:bir_stmt_t list |>`;
+val _ = Datatype `bir_stmt_end_t =
+  | BStmt_Jmp     bir_label_t
+  | BStmt_CJmp    bir_exp_t bir_label_t bir_label_t
+  | BStmt_Halt    bir_exp_t
+`;
+
+val _ = Datatype `bir_stmt_t =
+  | BStmtB bir_stmt_basic_t
+  | BStmtE bir_stmt_end_t
+`;
+
+val _ = Datatype `bir_block_t = <|
+  bb_label          : bir_label_t ;
+  bb_statements     : bir_stmt_basic_t list;
+  bb_last_statement : bir_stmt_end_t |>`;
+
 val _ = Datatype `bir_program_t = BirProgram (bir_block_t list)`;
 val _ = Datatype `bir_programcounter_t = <| bpc_label:bir_label_t; bpc_index:num |>`;
 
 val bir_pc_ss = rewrites (type_rws ``:bir_programcounter_t``);
 
-val _ = Datatype `bir_status_finished_t =
-    BSTF_Halted bir_val_t
-  | BSTF_ReachedEnd (bir_label_t option)`;
-
 val _ = Datatype `bir_status_t =
-    BST_Running (* BIR program is still running *)
-  | BST_Failed  (* BIR program execution failed *)
-  | BST_AssumptionViolated (* BIR program execution aborted, because assumption was violated *)
-  | BST_Finished bir_status_finished_t (* BIR program terminated successfully *)`
+    BST_Running                  (* BIR program is still running *)
+  | BST_Failed                   (* BIR program execution failed *)
+  | BST_AssumptionViolated       (* BIR program execution aborted, because assumption was violated *)
+  | BST_Halted bir_val_t        (* Halt called *)
+  | BST_JumpOutside bir_label_t (* Jump to unknown label *)`;
 
 val _ = Datatype `bir_state_t = <|
   bst_pc       : bir_programcounter_t;
@@ -50,24 +60,23 @@ val _ = Datatype `bir_state_t = <|
 |>`;
 
 val bir_state_ss = rewrites (type_rws ``:bir_state_t``);
-val bir_status_ss = rewrites ((type_rws ``:bir_status_t``) @ (type_rws ``:bir_status_finished_t``));
+val bir_status_ss = rewrites (type_rws ``:bir_status_t``);
 
+val bir_stmt_ss = rewrites ((type_rws ``:bir_stmt_t``) @ (type_rws ``:bir_stmt_end_t``) @
+                            (type_rws ``:bir_stmt_basic_t``));
 
 (* ------------------------------------------------------------------------- *)
 (* Programs                                                                  *)
 (* ------------------------------------------------------------------------- *)
 
-val bir_block_stmts_count_def = Define `bir_block_stmts_count bl = LENGTH bl.bb_statements`;
-val bir_program_stmts_count_def = Define`bir_program_stmts_count (BirProgram p) = SUM (MAP bir_block_stmts_count p)`;
-
 val bir_labels_of_program_def = Define `bir_labels_of_program (BirProgram p) =
   MAP (\bl. bl.bb_label) p`;
 
 val bir_is_valid_labels_def = Define `bir_is_valid_labels p =
-  ALL_DISTINCT (bir_labels_of_program p) /\ ~(MEM (BL_Label "") (bir_labels_of_program p))`;
+  ALL_DISTINCT (bir_labels_of_program p)`;
 
 val bir_is_valid_program_def = Define `bir_is_valid_program p <=>
-   (bir_is_valid_labels p /\ bir_program_stmts_count p > 0)`;
+   (bir_is_valid_labels p) /\ ~(p = BirProgram [])`;
 
 
 val bir_is_valid_labels_blocks_EQ_EL = store_thm ("bir_is_valid_labels_blocks_EQ_EL",
@@ -87,7 +96,6 @@ val bir_is_valid_labels_blocks_EQ = store_thm ("bir_is_valid_labels_blocks_EQ",
                 (bl1.bb_label = bl2.bb_label)) ==> (bl1 = bl2)``,
 
 METIS_TAC [listTheory.MEM_EL, bir_is_valid_labels_blocks_EQ_EL]);
-
 
 
 val bir_get_program_block_info_by_label_def = Define `bir_get_program_block_info_by_label
@@ -148,33 +156,15 @@ Cases_on `bir_get_program_block_info_by_label (BirProgram p) l` >| [
 
 val bir_is_valid_pc_def = Define `bir_is_valid_pc p pc =
    (?i bl. (bir_get_program_block_info_by_label p (pc.bpc_label) = SOME (i, bl)) /\
-           (pc.bpc_index < LENGTH bl.bb_statements))`;
-
-val bir_is_end_pc_def = Define `bir_is_end_pc (BirProgram p) pc =
-   (?i bl. (bir_get_program_block_info_by_label (BirProgram p) (pc.bpc_label) = SOME (i, bl)) /\
-           (pc.bpc_index = LENGTH bl.bb_statements) /\
-      (!j. (i < j /\ j < LENGTH p) ==> (((EL j p).bb_statements) = [])))`;
-
-val bir_is_allowed_pc_def = Define `bir_is_allowed_pc p pc =
-   (?i bl. (bir_get_program_block_info_by_label p (pc.bpc_label) = SOME (i, bl)) /\
            (pc.bpc_index <= LENGTH bl.bb_statements))`;
-
-
-val bir_is_valid_pc_not_end = store_thm ("bir_is_valid_pc_not_end",
-  ``!p pc. bir_is_valid_pc p pc ==> ~(bir_is_end_pc p pc)``,
-Cases >> rename1 `BirProgram p` >>
-SIMP_TAC arith_ss [bir_is_valid_pc_def, bir_is_end_pc_def,
-  GSYM LEFT_FORALL_IMP_THM]);
-
 
 val bir_is_valid_pc_of_valid_blocks = store_thm ("bir_is_valid_pc_of_valid_blocks",
   ``!p pc. bir_is_valid_labels (BirProgram p) ==>
            (bir_is_valid_pc (BirProgram p) pc <=> (?bl. MEM bl p /\ (pc.bpc_label = bl.bb_label) /\
-             (pc.bpc_index < LENGTH bl.bb_statements)))``,
+             (pc.bpc_index <= LENGTH bl.bb_statements)))``,
 SIMP_TAC std_ss [bir_is_valid_pc_def, bir_get_program_block_info_by_label_valid_THM,
   listTheory.MEM_EL, GSYM LEFT_EXISTS_AND_THM] >>
 METIS_TAC[]);
-
 
 
 val bir_get_program_block_info_by_label_valid_pc = store_thm ("bir_get_program_block_info_by_label_valid_pc",
@@ -184,7 +174,7 @@ SIMP_TAC std_ss [bir_is_valid_pc_def, GSYM LEFT_FORALL_IMP_THM]);
 
 val bir_get_current_statement_def = Define `bir_get_current_statement p pc =
   option_CASE (bir_get_program_block_info_by_label p pc.bpc_label) NONE
-     (\ (_, bl). if (pc.bpc_index < LENGTH bl.bb_statements) then SOME (EL (pc.bpc_index) bl.bb_statements) else NONE) `;
+     (\ (_, bl). if (pc.bpc_index < LENGTH bl.bb_statements) then SOME (BStmtB (EL (pc.bpc_index) bl.bb_statements)) else (if pc.bpc_index = LENGTH bl.bb_statements then SOME (BStmtE bl.bb_last_statement) else NONE))`;
 
 
 val bir_get_current_statement_IS_SOME = store_thm ("bir_get_current_statement_IS_SOME",
@@ -194,281 +184,70 @@ REPEAT GEN_TAC >>
 Cases_on `bir_get_program_block_info_by_label p pc.bpc_label` >> (
   ASM_SIMP_TAC std_ss [bir_get_current_statement_def, bir_is_valid_pc_def]
 ) >>
-SIMP_TAC (std_ss++QI_ss++pairSimps.gen_beta_ss++boolSimps.LIFT_COND_ss) []);
+SIMP_TAC (arith_ss++QI_ss++pairSimps.gen_beta_ss++boolSimps.LIFT_COND_ss) []);
 
 
-val bir_pc_normalise_def = Define `
-  (bir_pc_normalise (BirProgram p) pc = case bir_get_program_block_info_by_label (BirProgram p) (pc.bpc_label) of
-        SOME (n, bl) => if (pc.bpc_index < LENGTH bl.bb_statements)
-          then SOME pc
-          else (
-            let p' = FILTER (\bl. bl.bb_statements <> []) (DROP (SUC n) p) in
-            case p' of
-              | [] => NONE
-              | (bl'::_) => SOME <| bpc_label := bl'.bb_label ; bpc_index := 0 |>
-            )
-      | _ => NONE
-  )
-`;
+
+val bir_get_current_statement_SOME_B = store_thm ("bir_get_current_statement_SOME_B",
+  ``!p pc stmt. (bir_get_current_statement p pc = SOME (BStmtB stmt)) <=>
+                (?i bl. (bir_get_program_block_info_by_label p pc.bpc_label = SOME (i, bl)) /\
+                   (pc.bpc_index < LENGTH bl.bb_statements) /\
+                   (stmt = EL pc.bpc_index bl.bb_statements))``,
+
+REPEAT GEN_TAC >>
+Cases_on `bir_get_program_block_info_by_label p pc.bpc_label` >> (
+  ASM_SIMP_TAC std_ss [bir_get_current_statement_def]
+) >>
+SIMP_TAC (arith_ss++QI_ss++pairSimps.gen_beta_ss++boolSimps.LIFT_COND_ss++bir_stmt_ss) [] >>
+METIS_TAC[]);
+
+
+val bir_get_current_statement_SOME_E = store_thm ("bir_get_current_statement_SOME_E",
+  ``!p pc stmt. (bir_get_current_statement p pc = SOME (BStmtE stmt)) <=>
+                (?i bl. (bir_get_program_block_info_by_label p pc.bpc_label = SOME (i, bl)) /\
+                   (pc.bpc_index = LENGTH bl.bb_statements) /\
+                   (stmt = bl.bb_last_statement))``,
+
+REPEAT GEN_TAC >>
+Cases_on `bir_get_program_block_info_by_label p pc.bpc_label` >> (
+  ASM_SIMP_TAC std_ss [bir_get_current_statement_def]
+) >>
+SIMP_TAC (arith_ss++QI_ss++pairSimps.gen_beta_ss++boolSimps.LIFT_COND_ss++bir_stmt_ss++boolSimps.EQUIV_EXTRACT_ss) []);
 
 
 val bir_pc_next_def = Define `
-  bir_pc_next p pc = bir_pc_normalise p (pc with bpc_index updated_by SUC)`;
+  bir_pc_next pc = pc with bpc_index updated_by SUC`;
+
+val bir_block_pc_def = Define `bir_block_pc l = <| bpc_label := l; bpc_index := 0 |>`
 
 
-val bir_pc_normalise_EQ_SOME = store_thm ("bir_pc_normalise_EQ_SOME",
-``!p pc i bl pc'. (bir_get_program_block_info_by_label (BirProgram p) (pc.bpc_label) = SOME (i, bl)) ==>
-             ((bir_pc_normalise (BirProgram p) pc = SOME pc') <=>
-                (if (pc.bpc_index < LENGTH bl.bb_statements) then (pc' = pc) else
-                (?j. (i < j /\ j < LENGTH p /\ ((EL j p).bb_statements <> []) /\
-                     (pc' = <| bpc_label := (EL j p).bb_label; bpc_index := 0 |>) /\
-                     (!j'. (i < j' /\ j' < j) ==> (((EL j' p).bb_statements) = []))))))``,
+val bir_is_valid_pc_block_pc = store_thm ("bir_is_valid_pc_block_pc",
+``!l p. bir_is_valid_pc p (bir_block_pc l) <=>
+        MEM l (bir_labels_of_program p)``,
 
-SIMP_TAC std_ss [bir_pc_normalise_def, pairTheory.pair_case_thm] >>
-REPEAT STRIP_TAC >>
-Cases_on `pc.bpc_index < LENGTH bl.bb_statements` >- (
-  ASM_SIMP_TAC arith_ss [] >> METIS_TAC[]
-) >>
-ASM_SIMP_TAC std_ss [LET_DEF] >>
-Cases_on `FILTER (\bl. bl.bb_statements <> []) (DROP (SUC i) p)` >| [
-  ASM_SIMP_TAC list_ss [LET_DEF] >>
-  CCONTR_TAC >>
-  FULL_SIMP_TAC std_ss [] >>
-  `MEM (EL j p) (DROP (SUC i) p)` by (
-     SIMP_TAC (list_ss++boolSimps.CONJ_ss) [listTheory.MEM_EL, rich_listTheory.EL_DROP] >>
-     Q.EXISTS_TAC `j - SUC i` >>
-     ASM_SIMP_TAC arith_ss []
-  ) >>
-  `~(MEM (EL j p) (FILTER (\bl. bl.bb_statements <> []) (DROP (SUC i) p)))` by
-    ASM_SIMP_TAC list_ss [] >>
-  FULL_SIMP_TAC list_ss [listTheory.MEM_FILTER] >>
-  FULL_SIMP_TAC std_ss [],
-
-
-  rename1 `FILTER _ _ = bl0::bls` >>
-  ASM_SIMP_TAC list_ss [LET_DEF] >>
-  `?p1 p2. (LENGTH p1 = SUC i) /\ (p = p1 ++ p2)` by (
-     Q.EXISTS_TAC `TAKE (SUC i) p` >>
-     Q.EXISTS_TAC `DROP (SUC i) p` >>
-     FULL_SIMP_TAC list_ss [bir_get_program_block_info_by_label_THM]
-  ) >>
-  FULL_SIMP_TAC list_ss [rich_listTheory.DROP_APPEND1, listTheory.DROP_LENGTH_TOO_LONG] >>
-  Q.PAT_X_ASSUM `p = _ ++ _` (K ALL_TAC) >>
-  Q.PAT_X_ASSUM `_ = SOME _` (K ALL_TAC) >>
-  Induct_on `p2` >- ASM_SIMP_TAC list_ss [] >>
-  CONV_TAC (RENAME_VARS_CONV ["bl1"]) >>
-  REPEAT STRIP_TAC >>
-  Cases_on `(bl1.bb_statements) <> []` >> FULL_SIMP_TAC list_ss [] >| [
-    REPEAT (BasicProvers.VAR_EQ_TAC) >>
-    EQ_TAC >> REPEAT STRIP_TAC >> REPEAT BasicProvers.VAR_EQ_TAC >> ASM_SIMP_TAC list_ss [] >| [
-      Q.EXISTS_TAC `SUC i` >>
-      ASM_SIMP_TAC (list_ss++QI_ss) [rich_listTheory.EL_APPEND2],
-
-      Cases_on `j = SUC i` >- ASM_SIMP_TAC list_ss [rich_listTheory.EL_APPEND2] >>
-      Q.PAT_X_ASSUM `!j'. _` (MP_TAC o Q.SPEC `SUC i`) >>
-      ASM_SIMP_TAC list_ss [rich_listTheory.EL_APPEND2]
-    ],
-
-    EQ_TAC >> STRIP_TAC >> REPEAT BasicProvers.VAR_EQ_TAC >| [
-      Q.EXISTS_TAC `SUC j` >>
-      Q.PAT_X_ASSUM `_ <> []` MP_TAC >>
-      Q.PAT_X_ASSUM `!j. _` MP_TAC >>
-      `j - i = SUC (j - SUC i)` by DECIDE_TAC >>
-      ASM_SIMP_TAC list_ss [rich_listTheory.EL_APPEND2] >>
-      REPEAT STRIP_TAC >>
-      Cases_on `j' = SUC i` >- ASM_SIMP_TAC list_ss [] >>
-      Q.PAT_X_ASSUM `!j. _` (MP_TAC o Q.SPEC `PRE j'`) >>
-      `j' - SUC i = SUC (PRE j' - SUC i)` by DECIDE_TAC >>
-      ASM_SIMP_TAC list_ss [],
-
-      Q.EXISTS_TAC `PRE j` >>
-      Q.PAT_X_ASSUM `_ <> []` MP_TAC >>
-      Q.PAT_X_ASSUM `!j. _` MP_TAC >>
-
-      Cases_on `j = SUC i` >- ASM_SIMP_TAC list_ss [rich_listTheory.EL_APPEND2] >>
-      `j - SUC i = SUC (PRE j - SUC i)` by DECIDE_TAC >>
-      ASM_SIMP_TAC list_ss [rich_listTheory.EL_APPEND2] >>
-      REPEAT STRIP_TAC >>
-      Q.PAT_X_ASSUM `!j. _` (MP_TAC o Q.SPEC `SUC j'`) >>
-      `j' - i = SUC (j' - SUC i)` by DECIDE_TAC >>
-      ASM_SIMP_TAC list_ss []
-    ]
-  ]
-]);
-
-
-val bir_pc_normalise_EQ_NONE = store_thm ("bir_pc_normalise_EQ_NONE",
-``!p pc i bl. (bir_get_program_block_info_by_label (BirProgram p) (pc.bpc_label) = SOME (i, bl)) ==>
-             ((bir_pc_normalise (BirProgram p) pc = NONE) <=> (
-                (LENGTH bl.bb_statements <= pc.bpc_index) /\
-                (!j. (i < j /\ j < LENGTH p) ==> (((EL j p).bb_statements) = []))))``,
-
-SIMP_TAC std_ss [bir_pc_normalise_def, pairTheory.pair_case_thm] >>
-REPEAT STRIP_TAC >>
-Cases_on `pc.bpc_index < LENGTH bl.bb_statements` >> (
-  ASM_SIMP_TAC arith_ss []
-) >>
-Cases_on `FILTER (\bl. bl.bb_statements <> []) (DROP (SUC i) p)` >| [
-  ASM_SIMP_TAC list_ss [LET_DEF] >>
-  REPEAT STRIP_TAC >>
-  `MEM (EL j p) (DROP (SUC i) p)` by (
-     SIMP_TAC (list_ss++boolSimps.CONJ_ss) [listTheory.MEM_EL, rich_listTheory.EL_DROP] >>
-     Q.EXISTS_TAC `j - SUC i` >>
-     ASM_SIMP_TAC arith_ss []
-  ) >>
-  `~(MEM (EL j p) (FILTER (\bl. bl.bb_statements <> []) (DROP (SUC i) p)))` by
-    ASM_SIMP_TAC list_ss [] >>
-  FULL_SIMP_TAC list_ss [listTheory.MEM_FILTER] >>
-  FULL_SIMP_TAC std_ss [],
-
-
-  rename1 `FILTER _ _ = bl0::bls` >>
-  ASM_SIMP_TAC list_ss [LET_DEF] >>
-  `MEM bl0 (FILTER (\bl. bl.bb_statements <> []) (DROP (SUC i) p))` by
-    ASM_SIMP_TAC list_ss [] >>
-  POP_ASSUM MP_TAC >>
-  FULL_SIMP_TAC list_ss [listTheory.MEM_FILTER] >>
-  SIMP_TAC (list_ss++boolSimps.CONJ_ss) [listTheory.MEM_EL, rich_listTheory.EL_DROP] >>
-  REPEAT STRIP_TAC >>
-  rename1 `bl0 = EL (n + SUC i) p` >>
-  Q.EXISTS_TAC `n + SUC i` >>
-  FULL_SIMP_TAC list_ss []
-]);
-
-
-val bir_pc_normalise_EQ_NONE_not_is_valid = store_thm ("bir_pc_normalise_EQ_NONE_not_is_valid",
-``!p pc. (bir_pc_normalise p pc = NONE) ==> (
-         ~(bir_is_valid_pc p pc))``,
-
-Cases_on `p` >> rename1 `BirProgram p` >>
-REPEAT STRIP_TAC >>
-FULL_SIMP_TAC std_ss [bir_is_valid_pc_def, bir_pc_normalise_def] >>
-FULL_SIMP_TAC std_ss [pairTheory.pair_case_thm]);
-
-
-val bir_pc_normalise_EQ_NONE_is_end_pc = store_thm ("bir_pc_normalise_EQ_NONE_is_end_pc",
-``!p pc. bir_is_allowed_pc p pc ==>
-         ((bir_pc_normalise p pc = NONE) <=> (
-           bir_is_end_pc p pc))``,
-
-Cases_on `p` >> rename1 `BirProgram p` >>
-SIMP_TAC std_ss [bir_is_allowed_pc_def, GSYM LEFT_FORALL_IMP_THM] >>
-REPEAT STRIP_TAC >>
-MP_TAC (Q.SPECL [`p`, `pc`] bir_pc_normalise_EQ_NONE) >>
-FULL_SIMP_TAC (arith_ss++boolSimps.EQUIV_EXTRACT_ss) [bir_is_end_pc_def]);
-
-
-
-val bir_is_allowed_pc_inc_valid = store_thm ("bir_is_allowed_pc_inc_valid",
-``!p pc. bir_is_valid_pc p pc ==> bir_is_allowed_pc p (pc with bpc_index updated_by SUC)``,
-
-SIMP_TAC (arith_ss++bir_pc_ss) [bir_is_valid_pc_def, bir_is_allowed_pc_def, GSYM LEFT_FORALL_IMP_THM]);
-
-val bir_is_allowed_pc_jmp = store_thm ("bir_is_allowed_pc_jmp",
-``!l p. MEM l (bir_labels_of_program p) ==>
-        bir_is_allowed_pc p <| bpc_label := l; bpc_index := 0 |>``,
-
-SIMP_TAC (std_ss++bir_pc_ss) [bir_is_allowed_pc_def, GSYM bir_get_program_block_info_by_label_MEM]);
-
-
-val bir_pc_normalise_valid = store_thm ("bir_pc_normalise_valid",
-``!p pc pc'. (bir_is_valid_labels p /\ (MEM pc.bpc_label (bir_labels_of_program p)) /\
-              (bir_pc_normalise p pc = SOME pc')) ==>
-             (bir_is_valid_pc p pc')``,
-
-Cases >> rename1 `BirProgram p` >>
-SIMP_TAC list_ss [bir_labels_of_program_def, bir_pc_normalise_EQ_SOME,
-  listTheory.MEM_MAP, GSYM RIGHT_EXISTS_AND_THM] >>
-REPEAT STRIP_TAC >>
-FULL_SIMP_TAC std_ss [listTheory.MEM_EL] >>
-rename1 `bl = EL i p` >>
-`bir_get_program_block_info_by_label (BirProgram p) pc.bpc_label = SOME (i, bl)` by
-  METIS_TAC[bir_get_program_block_info_by_label_valid_THM] >>
-
-MP_TAC (Q.SPECL [`p`, `pc`, `i`, `bl`, `pc'`] bir_pc_normalise_EQ_SOME) >>
-FULL_SIMP_TAC std_ss [bir_is_valid_pc_def] >>
-Cases_on `pc.bpc_index < LENGTH (EL i p).bb_statements` >| [
-  ASM_SIMP_TAC std_ss [] >> METIS_TAC[],
-
-  ASM_SIMP_TAC (std_ss++bir_pc_ss) [bir_get_program_block_info_by_label_valid_THM,
-    GSYM LEFT_FORALL_IMP_THM] >>
-  REPEAT STRIP_TAC >>
-  Q.EXISTS_TAC `j` >>
-  ASM_SIMP_TAC arith_ss [] >>
-  Cases_on `(EL j p).bb_statements` >> FULL_SIMP_TAC list_ss []
-]);
+SIMP_TAC (std_ss++bir_pc_ss) [bir_is_valid_pc_def,
+  bir_get_program_block_info_by_label_MEM, bir_block_pc_def]);
 
 
 val bir_pc_next_valid = store_thm ("bir_pc_next_valid",
-``!p pc pc'. (bir_is_valid_labels p /\ bir_is_valid_pc p pc /\ (bir_pc_next p pc = SOME pc')) ==>
-             (bir_is_valid_pc p pc')``,
+``!p pc. (bir_is_valid_pc p (bir_pc_next pc)) <=>
+         (?stmt. bir_get_current_statement p pc = SOME (BStmtB stmt))``,
 
 REPEAT STRIP_TAC >>
-MATCH_MP_TAC bir_pc_normalise_valid >>
-Q.EXISTS_TAC `pc with bpc_index updated_by SUC` >>
-Cases_on `p` >>
-FULL_SIMP_TAC (std_ss++bir_pc_ss) [bir_pc_next_def, bir_is_valid_pc_def, bir_labels_of_program_def,
-  listTheory.MEM_MAP] >>
-METIS_TAC[listTheory.MEM_EL, bir_get_program_block_info_by_label_valid_THM]);
-
+SIMP_TAC (std_ss++bir_pc_ss) [bir_is_valid_pc_def, bir_pc_next_def,
+  bir_get_current_statement_SOME_B, GSYM arithmeticTheory.LESS_EQ]);
 
 val bir_pc_first_def = Define
-  `bir_pc_first (BirProgram p) = let bl = HD (FILTER (\bl. (bl.bb_statements) <> []) p) in
-    (<| bpc_label := bl.bb_label; bpc_index := 0 |>):bir_programcounter_t`;
-
-val bir_pc_last_def = Define
-  `bir_pc_last (BirProgram p) = let bl = LAST (FILTER (\bl. (bl.bb_statements) <> []) p) in
-    (<| bpc_label := bl.bb_label; bpc_index := LENGTH bl.bb_statements - 1 |>):bir_programcounter_t`;
-
-
-val bir_program_stmts_count_FILTER_NEQ_NIL = store_thm ("bir_program_stmts_count_FILTER_NEQ_NIL",
-  ``!p. (bir_program_stmts_count (BirProgram p) > 0) ==>
-    (?bl0 bls. (FILTER (\bl. bl.bb_statements <> []) p = bl0 :: bls) /\
-              EVERY (\bl. (bl.bb_statements <> []) /\ MEM bl p) (bl0::bls))``,
-
-Induct_on `p` >> (
-  FULL_SIMP_TAC list_ss [bir_program_stmts_count_def, bir_block_stmts_count_def]
-) >>
-CONV_TAC (RENAME_VARS_CONV ["bl"]) >> GEN_TAC >>
-Cases_on `bl.bb_statements` >| [
-  SIMP_TAC list_ss [] >>
-  REPEAT STRIP_TAC >>
-  FULL_SIMP_TAC list_ss [listTheory.EVERY_MEM],
-
-  SIMP_TAC list_ss [listTheory.EVERY_FILTER] >>
-  ASM_SIMP_TAC list_ss [listTheory.EVERY_MEM]
-]);
-
+  `bir_pc_first (BirProgram p) = bir_block_pc (HD p).bb_label`;
 
 val bir_pc_first_valid = store_thm ("bir_pc_first_valid",
   ``!p. bir_is_valid_program p ==> bir_is_valid_pc p (bir_pc_first p)``,
 
 Cases >> rename1 `BirProgram p` >>
-SIMP_TAC (std_ss++bir_pc_ss) [bir_is_valid_pc_of_valid_blocks, bir_is_valid_program_def,
-  bir_pc_first_def, LET_DEF] >>
-ASSUME_TAC (Q.SPEC `p` bir_program_stmts_count_FILTER_NEQ_NIL) >>
-REPEAT STRIP_TAC >>
-FULL_SIMP_TAC list_ss [] >>
-rename1 `bl0.bb_statements <> []` >>
-Q.EXISTS_TAC `bl0` >>
-Cases_on `bl0.bb_statements` >> FULL_SIMP_TAC list_ss []);
-
-
-val bir_pc_last_valid = store_thm ("bir_pc_last_valid",
-  ``!p. bir_is_valid_program p ==> bir_is_valid_pc p (bir_pc_last p)``,
-
-Cases >> rename1 `BirProgram p` >>
-SIMP_TAC (std_ss++bir_pc_ss) [bir_is_valid_pc_of_valid_blocks, bir_is_valid_program_def,
-  bir_pc_last_def, LET_DEF] >>
-ASSUME_TAC (Q.SPEC `p` bir_program_stmts_count_FILTER_NEQ_NIL) >>
-REPEAT STRIP_TAC >>
-FULL_SIMP_TAC list_ss [] >>
-rename1 `FILTER _ p = bl0::bls` >>
-Q.EXISTS_TAC `LAST (bl0::bls)` >>
-`MEM (LAST (bl0::bls)) (bl0::bls)` by MATCH_ACCEPT_TAC rich_listTheory.MEM_LAST >>
-ASM_SIMP_TAC arith_ss [rich_listTheory.LENGTH_NOT_NULL, listTheory.NULL_EQ] >>
-FULL_SIMP_TAC list_ss [listTheory.EVERY_MEM]);
-
+SIMP_TAC std_ss [bir_pc_first_def, bir_is_valid_pc_block_pc] >>
+Cases_on `p` >> (
+  SIMP_TAC list_ss [bir_is_valid_program_def, bir_labels_of_program_def]
+));
 
 
 val bir_is_valid_pc_label_OK = store_thm ("bir_is_valid_pc_label_OK",
@@ -480,55 +259,6 @@ SIMP_TAC std_ss [bir_is_valid_pc_def, listTheory.MEM_MAP,
   bir_get_program_block_info_by_label_THM] >>
 SIMP_TAC std_ss [listTheory.MEM_EL, GSYM RIGHT_EXISTS_AND_THM] >>
 METIS_TAC[]);
-
-
-val bir_pc_next_valid_EQ_NONE = store_thm ("bir_pc_next_valid_EQ_NONE",
-``!p pc. (bir_is_valid_labels p /\ bir_is_valid_pc p pc) ==>
-          ((bir_pc_next p pc = NONE) <=> (pc = bir_pc_last p))``,
-
-REPEAT STRIP_TAC >>
-ASM_SIMP_TAC std_ss [bir_pc_next_def,
-  bir_pc_normalise_EQ_NONE_is_end_pc, bir_is_allowed_pc_inc_valid] >>
-
-Cases_on `p` >> rename1 `BirProgram p` >>
-ASM_SIMP_TAC (std_ss++bir_pc_ss) [bir_pc_last_def, LET_THM, bir_is_end_pc_def] >>
-
-`FILTER (\bl. bl.bb_statements <> []) p <> []` by (
-  STRIP_TAC  >>
-  FULL_SIMP_TAC std_ss [bir_is_valid_pc_def, bir_get_program_block_info_by_label_THM] >>
-  `MEM (EL i p) (FILTER (\bl. bl.bb_statements <> []) p)` suffices_by ASM_SIMP_TAC list_ss [] >>
-  SIMP_TAC list_ss [listTheory.MEM_FILTER, listTheory.MEM_EL] >>
-  REPEAT STRIP_TAC >| [
-    Cases_on `(EL i p).bb_statements` >> FULL_SIMP_TAC list_ss [],
-    METIS_TAC[]
-  ]
-) >>
-
-IMP_RES_TAC LAST_FILTER_EL >>
-FULL_SIMP_TAC (list_ss++bir_pc_ss) [DB.fetch "-" "bir_programcounter_t_component_equality",
-  bir_is_valid_pc_def] >>
-REV_FULL_SIMP_TAC std_ss [bir_get_program_block_info_by_label_valid_THM] >>
-EQ_TAC >> STRIP_TAC >| [
-  `~(i < i')` by (
-    STRIP_TAC >>
-    `bl.bb_statements = []` by METIS_TAC[] >>
-    FULL_SIMP_TAC list_ss []
-  ) >>
-  `~(i' < i)` by (
-    STRIP_TAC >>
-    `(EL i p).bb_statements = []` by METIS_TAC[] >>
-    FULL_SIMP_TAC list_ss []
-  ) >>
-  `i' = i` by DECIDE_TAC >>
-  FULL_SIMP_TAC arith_ss [],
-
-  `bl = EL i p` by METIS_TAC [bir_is_valid_labels_blocks_EQ, listTheory.MEM_EL] >>
-  `i' = i` by METIS_TAC [bir_is_valid_labels_blocks_EQ_EL] >>
-  FULL_SIMP_TAC arith_ss [] >>
-  REPEAT STRIP_TAC >>
-  `~(LENGTH (EL j p).bb_statements > 0)` by METIS_TAC[] >>
-  ASM_SIMP_TAC arith_ss []
-]);
 
 
 
@@ -554,17 +284,6 @@ val bir_state_set_failed_is_failed = store_thm ("bir_state_set_failed_is_failed"
   ``!st. bir_state_is_failed (bir_state_set_failed st)``,
 SIMP_TAC (std_ss ++ bir_state_ss) [bir_state_set_failed_def, bir_state_is_failed_def]);
 
-val bir_state_normalise_pc_def = Define `bir_state_normalise_pc p (st:bir_state_t) =
-  case bir_pc_normalise p st.bst_pc of
-    | SOME pc' => (st with bst_pc := pc')
-    | NONE => (st with bst_status := BST_Finished (BSTF_ReachedEnd NONE))`;
-
-val bir_state_incr_pc_def = Define `bir_state_incr_pc p (st:bir_state_t) =
-  bir_state_normalise_pc p (st with bst_pc := (st.bst_pc with bpc_index updated_by SUC))`
-
-val bir_state_set_pc_def = Define `bir_state_set_pc p (st:bir_state_t) pc' =
-  bir_state_normalise_pc p (st with bst_pc := pc')`;
-
 val bir_state_init_def = Define `bir_state_init p = <|
     bst_pc       := bir_pc_first p
   ; bst_environ  := bir_empty_env
@@ -582,27 +301,48 @@ val bir_declare_initial_value_def = Define `
   (bir_declare_initial_value (BType_Imm _) = NONE) /\
   (bir_declare_initial_value (BType_Mem at vt) = SOME (BVal_Mem at vt (K 0)))`;
 
-val bir_exec_stmt_declare_def = Define `bir_exec_stmt_declare p v ty (st : bir_state_t) =
+val bir_exec_stmt_declare_def = Define `bir_exec_stmt_declare v ty (st : bir_state_t) =
    if bir_env_varname_is_bound st.bst_environ v then
      bir_state_set_failed st
    else (
       case (bir_env_update v (bir_declare_initial_value ty) ty st.bst_environ) of
-        | SOME env => bir_state_incr_pc p (st with bst_environ := env)
-        | NONE => (* Cannot happen, since bir_declare_initial_value returns value of correct type *) ARB)`;
+        | SOME env => (st with bst_environ := env)
+        | NONE => (* Cannot happen, since bir_declare_initial_value returns value of correct type *)            bir_state_set_failed st)`;
 
-val bir_exec_stmt_assign_def = Define `bir_exec_stmt_assign p v ex (st : bir_state_t) =
+val bir_exec_stmt_assign_def = Define `bir_exec_stmt_assign v ex (st : bir_state_t) =
    let env_o = bir_env_write v (bir_eval_exp ex st.bst_environ) st.bst_environ in
    case env_o of
-     | SOME env => bir_state_incr_pc p (st with bst_environ := env)
+     | SOME env => (st with bst_environ := env)
      | NONE => bir_state_set_failed st`;
 
+val bir_exec_stmt_assert_def = Define `bir_exec_stmt_assert ex (st : bir_state_t) =
+  case (bir_dest_bool_val (bir_eval_exp ex st.bst_environ)) of
+    | SOME T => st
+    | SOME F => bir_state_set_failed st
+    | NONE => bir_state_set_failed st`
+
+val bir_exec_stmt_assume_def = Define `bir_exec_stmt_assume ex (st : bir_state_t) =
+  case (bir_dest_bool_val (bir_eval_exp ex st.bst_environ)) of
+    | SOME T => st
+    | SOME F => (st with bst_status := BST_AssumptionViolated)
+    | NONE => bir_state_set_failed st`;
+
+
+val bir_exec_stmtB_def = Define `
+  (bir_exec_stmtB (BStmt_Declare v) st = bir_exec_stmt_declare (bir_var_name v) (bir_var_type v) st) /\
+  (bir_exec_stmtB (BStmt_Assert ex) st = bir_exec_stmt_assert ex st) /\
+  (bir_exec_stmtB (BStmt_Assume ex) st = bir_exec_stmt_assume ex st) /\
+  (bir_exec_stmtB (BStmt_Assign v ex) st = bir_exec_stmt_assign v ex st)`;
+
+
+
 val bir_exec_stmt_halt_def = Define `bir_exec_stmt_halt ex (st : bir_state_t) =
-    (st with bst_status := BST_Finished (BSTF_Halted (bir_eval_exp ex st.bst_environ)))`;
+    (st with bst_status := BST_Halted (bir_eval_exp ex st.bst_environ))`;
 
 val bir_exec_stmt_jmp_def = Define `bir_exec_stmt_jmp p l (st : bir_state_t) =
     if (MEM l (bir_labels_of_program p)) then
-      bir_state_set_pc p st <| bpc_label := l; bpc_index := 0 |>
-    else (st with bst_status := (BST_Finished (BSTF_ReachedEnd (SOME l))))`;
+      st with bst_pc := bir_block_pc l
+    else (st with bst_status := (BST_JumpOutside l))`;
 
 val bir_exec_stmt_cjmp_def = Define `bir_exec_stmt_cjmp p ex l1 l2 (st : bir_state_t) =
   case (bir_dest_bool_val (bir_eval_exp ex st.bst_environ)) of
@@ -610,27 +350,18 @@ val bir_exec_stmt_cjmp_def = Define `bir_exec_stmt_cjmp p ex l1 l2 (st : bir_sta
     | SOME F => bir_exec_stmt_jmp p l2 st
     | NONE => bir_state_set_failed st`;
 
-val bir_exec_stmt_assert_def = Define `bir_exec_stmt_assert p ex (st : bir_state_t) =
-  case (bir_dest_bool_val (bir_eval_exp ex st.bst_environ)) of
-    | SOME T => bir_state_incr_pc p st
-    | SOME F => bir_state_set_failed st
-    | NONE => bir_state_set_failed st`
 
-val bir_exec_stmt_assume_def = Define `bir_exec_stmt_assume p ex (st : bir_state_t) =
-  case (bir_dest_bool_val (bir_eval_exp ex st.bst_environ)) of
-    | SOME T => bir_state_incr_pc p st
-    | SOME F => (st with bst_status := BST_AssumptionViolated)
-    | NONE => bir_state_set_failed st`;
+val bir_exec_stmtE_def = Define `
+  (bir_exec_stmtE p (BStmt_Jmp l) st = bir_exec_stmt_jmp p l st) /\
+  (bir_exec_stmtE p (BStmt_CJmp e l1 l2) st = bir_exec_stmt_cjmp p e l1 l2 st) /\
+  (bir_exec_stmtE p (BStmt_Halt ex) st = bir_exec_stmt_halt ex st)`;
 
 
 val bir_exec_stmt_def = Define `
-  (bir_exec_stmt p (BStmt_Jmp l) st = bir_exec_stmt_jmp p l st) /\
-  (bir_exec_stmt p (BStmt_CJmp e l1 l2) st = bir_exec_stmt_cjmp p e l1 l2 st) /\
-  (bir_exec_stmt p (BStmt_Declare v) st = bir_exec_stmt_declare p (bir_var_name v) (bir_var_type v) st) /\
-  (bir_exec_stmt p (BStmt_Assert ex) st = bir_exec_stmt_assert p ex st) /\
-  (bir_exec_stmt p (BStmt_Assume ex) st = bir_exec_stmt_assume p ex st) /\
-  (bir_exec_stmt p (BStmt_Assign v ex) st = bir_exec_stmt_assign p v ex st) /\
-  (bir_exec_stmt p (BStmt_Halt ex) st = bir_exec_stmt_halt ex st)`;
+  (bir_exec_stmt p (BStmtB bst) st =
+     let st' = bir_exec_stmtB bst st in
+     if (bir_state_is_failed st') then st else (st' with bst_pc updated_by bir_pc_next)) /\
+  (bir_exec_stmt p (BStmtE bst) st = bir_exec_stmtE p bst st)`;
 
 
 val bir_exec_step_def = Define `bir_exec_step p state =
@@ -646,8 +377,7 @@ val bir_exec_step_def = Define `bir_exec_step p state =
 (* ------------------------------------------------------------------------- *)
 
 val bir_is_valid_state_def = Define `bir_is_valid_state p st <=>
-  ((bir_is_well_typed_env st.bst_environ) /\ (if st.bst_status = BST_Finished (BSTF_ReachedEnd NONE) then bir_is_end_pc p st.bst_pc else
-      bir_is_valid_pc p st.bst_pc))`;
+  ((bir_is_well_typed_env st.bst_environ) /\ bir_is_valid_pc p st.bst_pc)`;
 
 val bir_state_init_valid = store_thm ("bir_state_init_valid",
   ``!p. bir_is_valid_program p ==> bir_is_valid_state p (bir_state_init p)``,
@@ -666,51 +396,25 @@ val bir_exec_step_valid_THM = store_thm ("bir_exec_step_valid_THM",
                      (bir_exec_step p st = (bir_exec_stmt p stmt st))))``,
 
 REPEAT STRIP_TAC >>
-SIMP_TAC std_ss [bir_exec_step_def] >>
+FULL_SIMP_TAC std_ss [bir_exec_step_def, bir_is_valid_state_def] >>
 Cases_on `bir_state_is_terminated st` >> ASM_SIMP_TAC (std_ss++boolSimps.CONJ_ss) [] >>
-`st.bst_status <> BST_Finished (BSTF_ReachedEnd NONE)` by (
-  STRIP_TAC >> FULL_SIMP_TAC (std_ss++bir_status_ss) [bir_state_is_terminated_def]
-) >>
-`?stm. bir_get_current_statement p st.bst_pc = SOME stm` by (
-  `IS_SOME (bir_get_current_statement p st.bst_pc)` suffices_by METIS_TAC[optionTheory.IS_SOME_EXISTS] >>
-  FULL_SIMP_TAC std_ss [bir_get_current_statement_IS_SOME,
-     bir_is_valid_state_def]
-) >>
-FULL_SIMP_TAC std_ss [bir_is_valid_state_def]);
+`IS_SOME (bir_get_current_statement p st.bst_pc)` suffices_by METIS_TAC[optionTheory.IS_SOME_EXISTS] >>
+FULL_SIMP_TAC std_ss [bir_get_current_statement_IS_SOME,
+  bir_is_valid_state_def]);
 
 
 val bir_is_valid_state_set_failed = store_thm ("bir_is_valid_state_set_failed",
-  ``!p st. bir_is_valid_state p st /\ bir_is_valid_pc p st.bst_pc ==>
+  ``!p st. bir_is_valid_state p st ==>
            bir_is_valid_state p (bir_state_set_failed st)``,
 SIMP_TAC (std_ss++bir_status_ss++bir_state_ss) [bir_is_valid_state_def, bir_state_set_failed_def]);
 
 
-val bir_is_valid_state_incr_pc = store_thm ("bir_is_valid_state_incr_pc",
-  ``!p st. bir_is_valid_program p /\ bir_is_valid_state p st /\ bir_is_valid_pc p st.bst_pc ==>
-           bir_is_valid_state p (bir_state_incr_pc p st)``,
-SIMP_TAC (std_ss++bir_state_ss++boolSimps.CONJ_ss) [bir_state_incr_pc_def, bir_is_valid_state_def,
-  bir_state_normalise_pc_def, bir_is_valid_pc_not_end
-] >>
-REPEAT GEN_TAC >> STRIP_TAC >>
-Cases_on `bir_pc_normalise p (st.bst_pc with bpc_index updated_by SUC)` >- (
-  ASM_SIMP_TAC (std_ss++bir_state_ss) [GSYM bir_pc_normalise_EQ_NONE_is_end_pc,
-    bir_is_allowed_pc_inc_valid]
-) >>
-rename1 `_ = SOME pc'` >>
-ASM_SIMP_TAC (std_ss++bir_pc_ss++bir_state_ss) [] >>
-MATCH_MP_TAC bir_pc_normalise_valid >>
-Q.EXISTS_TAC `st.bst_pc with bpc_index updated_by SUC` >>
-FULL_SIMP_TAC (std_ss++bir_pc_ss) [bir_is_valid_pc_label_OK,
-   bir_is_valid_program_def]);
-
-
-
-val bir_exec_step_valid_state_invar_declare = prove (
-  ``!p st v. (bir_is_valid_program p /\ bir_is_valid_state p st /\ bir_is_valid_pc p st.bst_pc) ==>
-             bir_is_valid_state p (bir_exec_stmt p (BStmt_Declare v) st)``,
+val bir_exec_stmtB_valid_state_invar_declare = prove (
+  ``!p st v. bir_is_valid_state p st ==>
+             bir_is_valid_state p (bir_exec_stmtB (BStmt_Declare v) st)``,
 
 Cases_on `v` >> rename1 `BVar v ty` >>
-SIMP_TAC (std_ss++boolSimps.LIFT_COND_ss) [bir_exec_stmt_def, bir_exec_stmt_declare_def, LET_THM,
+SIMP_TAC (std_ss++boolSimps.LIFT_COND_ss) [bir_exec_stmtB_def, bir_exec_stmt_declare_def, LET_THM,
   bir_is_valid_state_set_failed, bir_var_type_def, bir_var_name_def] >>
 REPEAT STRIP_TAC >>
 Cases_on `bir_env_varname_is_bound st.bst_environ v` >> ASM_REWRITE_TAC[] >>
@@ -721,136 +425,222 @@ Cases_on `bir_env_varname_is_bound st.bst_environ v` >> ASM_REWRITE_TAC[] >>
     FULL_SIMP_TAC std_ss [bir_declare_initial_value_def, type_of_bir_val_def, bir_env_update_def]
   )
 ) >>
-ASM_SIMP_TAC std_ss [] >>
-MATCH_MP_TAC bir_is_valid_state_incr_pc >>
 FULL_SIMP_TAC (std_ss++bir_state_ss) [bir_is_valid_state_def] >>
 METIS_TAC[bir_env_update_is_well_typed_env]);
 
 
 
-val bir_exec_step_valid_state_invar_assign = prove (
-  ``!p st v ex. (bir_is_valid_program p /\ bir_is_valid_state p st /\ bir_is_valid_pc p st.bst_pc) ==>
-                 bir_is_valid_state p (bir_exec_stmt p (BStmt_Assign v ex) st)``,
+val bir_exec_stmtB_valid_state_invar_assign = prove (
+  ``!p st v ex. bir_is_valid_state p st ==>
+                bir_is_valid_state p (bir_exec_stmtB (BStmt_Assign v ex) st)``,
 Cases_on `v` >> rename1 `BVar v ty` >>
 REPEAT STRIP_TAC >>
-SIMP_TAC std_ss [bir_exec_stmt_def, bir_exec_stmt_assign_def, LET_THM] >>
+SIMP_TAC std_ss [bir_exec_stmtB_def, bir_exec_stmt_assign_def, LET_THM] >>
 Cases_on `bir_env_write (BVar v ty) (bir_eval_exp ex st.bst_environ)
        st.bst_environ` >> (
   ASM_SIMP_TAC std_ss [bir_is_valid_state_set_failed]
 ) >>
-MATCH_MP_TAC bir_is_valid_state_incr_pc >>
-ASM_SIMP_TAC (std_ss++bir_state_ss) [] >>
 FULL_SIMP_TAC (std_ss++bir_state_ss) [bir_is_valid_state_def] >>
 METIS_TAC[bir_env_write_is_well_typed_env]);
 
 
-val bir_exec_step_valid_state_invar_jmp' = prove (
-  ``!p st l. (bir_is_valid_program p /\ bir_is_valid_state p st /\ bir_is_valid_pc p st.bst_pc) ==>
+val bir_exec_stmtB_valid_state_invar_assert = prove (
+  ``!p st ex. bir_is_valid_state p st ==>
+              bir_is_valid_state p (bir_exec_stmtB (BStmt_Assert ex) st)``,
+
+SIMP_TAC (std_ss++bir_state_ss++bir_status_ss) [bir_exec_stmtB_def, bir_exec_stmt_assert_def] >>
+REPEAT GEN_TAC >> STRIP_TAC >>
+REPEAT CASE_TAC >> (
+  ASM_SIMP_TAC std_ss [bir_is_valid_state_set_failed]
+));
+
+
+val bir_exec_stmtB_valid_state_invar_assume = prove (
+  ``!p st ex. bir_is_valid_state p st ==>
+              bir_is_valid_state p (bir_exec_stmtB (BStmt_Assume ex) st)``,
+
+SIMP_TAC (std_ss++bir_state_ss++bir_status_ss) [bir_exec_stmtB_def, bir_exec_stmt_assume_def] >>
+REPEAT GEN_TAC >> STRIP_TAC >>
+REPEAT CASE_TAC >> (
+  ASM_SIMP_TAC std_ss [bir_is_valid_state_set_failed]
+) >>
+FULL_SIMP_TAC (std_ss++bir_state_ss++bir_status_ss) [bir_is_valid_state_def]);
+
+
+val bir_exec_stmtB_valid_state_invar = store_thm ("bir_exec_stmtB_valid_state_invar",
+``!p st stmt. bir_is_valid_state p st ==>
+              bir_is_valid_state p (bir_exec_stmtB stmt st)``,
+
+REPEAT STRIP_TAC >>
+Cases_on `stmt` >> (
+  ASM_SIMP_TAC std_ss [
+    bir_exec_stmtB_valid_state_invar_declare,
+    bir_exec_stmtB_valid_state_invar_assign,
+    bir_exec_stmtB_valid_state_invar_assume,
+    bir_exec_stmtB_valid_state_invar_assert]
+));
+
+
+val bir_exec_stmtB_pc_unchanged = store_thm ("bir_exec_stmtB_pc_unchanged",
+``!p st stmt. (bir_exec_stmtB stmt st).bst_pc = st.bst_pc``,
+
+REPEAT STRIP_TAC >>
+Cases_on `stmt` >> (
+  ASM_SIMP_TAC std_ss [bir_exec_stmtB_def, LET_DEF,
+    bir_exec_stmt_declare_def, bir_exec_stmt_assume_def,
+    bir_exec_stmt_assign_def, bir_exec_stmt_assert_def] >>
+  REPEAT CASE_TAC >>
+  FULL_SIMP_TAC (std_ss++bir_state_ss) [bir_state_set_failed_def]
+));
+
+
+val bir_exec_stmtB_not_halted_jumped = store_thm ("bir_exec_stmtB_not_halted_jumped",
+``(!p st stmt l. (st.bst_status <> BST_JumpOutside l) ==> ((bir_exec_stmtB stmt st).bst_status <> BST_JumpOutside l)) /\
+  (!p st stmt v. (st.bst_status <> BST_Halted v) ==> ((bir_exec_stmtB stmt st).bst_status <> BST_Halted v))``,
+
+CONJ_TAC >> Cases_on `stmt` >> (
+  ASM_SIMP_TAC std_ss [bir_exec_stmtB_def, LET_DEF,
+    bir_exec_stmt_declare_def, bir_exec_stmt_assume_def,
+    bir_exec_stmt_assign_def, bir_exec_stmt_assert_def] >>
+  REPEAT GEN_TAC >> STRIP_TAC >>
+  REPEAT CASE_TAC >>
+  FULL_SIMP_TAC (std_ss++bir_state_ss++bir_status_ss) [bir_state_set_failed_def]
+));
+
+
+val bir_exec_stmtB_terminates_no_change = store_thm ("bir_exec_stmtB_terminates_no_change",
+``!p st stmt. ~(bir_state_is_terminated st) ==>
+              (bir_state_is_terminated (bir_exec_stmtB stmt st)) ==>
+              (((bir_exec_stmtB stmt st) with bst_status := BST_Running) = st)``,
+
+SIMP_TAC (std_ss++bir_state_ss) [bir_state_is_terminated_def,
+  DB.fetch "-" "bir_state_t_component_equality", bir_exec_stmtB_pc_unchanged] >>
+Cases_on `stmt` >> (
+  SIMP_TAC std_ss [bir_exec_stmtB_def, LET_DEF,
+    bir_exec_stmt_declare_def, bir_exec_stmt_assume_def,
+    bir_exec_stmt_assign_def, bir_exec_stmt_assert_def] >>
+  REPEAT GEN_TAC >> STRIP_TAC >>
+  REPEAT CASE_TAC >>
+  FULL_SIMP_TAC (std_ss++bir_state_ss++bir_status_ss) [bir_state_set_failed_def,
+    bir_state_is_terminated_def]
+));
+
+
+
+val bir_exec_stmtE_valid_state_invar_jmp' = prove (
+  ``!p st l. bir_is_valid_state p st ==>
              bir_is_valid_state p (bir_exec_stmt_jmp p l st)``,
 SIMP_TAC std_ss [bir_exec_stmt_jmp_def] >>
 REPEAT STRIP_TAC >>
 COND_CASES_TAC >| [
-  ASM_SIMP_TAC (std_ss++bir_state_ss) [bir_is_valid_state_def, bir_state_set_pc_def,
-    bir_state_normalise_pc_def] >>
-  Cases_on `bir_pc_normalise p <|bpc_label := l; bpc_index := 0|>` >| [
-    FULL_SIMP_TAC (std_ss++bir_state_ss) [bir_is_valid_state_def] >>
-    ASM_SIMP_TAC std_ss [GSYM bir_pc_normalise_EQ_NONE_is_end_pc,
-      bir_is_allowed_pc_jmp],
-
-    rename1 `_ = SOME pc'` >>
-    FULL_SIMP_TAC (std_ss++bir_pc_ss++bir_state_ss) [bir_is_valid_state_def,
-      bir_is_valid_pc_not_end] >>
-    MATCH_MP_TAC bir_pc_normalise_valid >>
-    Q.EXISTS_TAC `<| bpc_label := l; bpc_index := 0|>` >>
-    FULL_SIMP_TAC (std_ss++bir_pc_ss) [bir_is_valid_program_def]
-  ],
+  FULL_SIMP_TAC (std_ss++bir_state_ss) [bir_is_valid_state_def,
+    bir_is_valid_pc_block_pc],
 
   FULL_SIMP_TAC (std_ss++bir_state_ss++bir_status_ss) [bir_is_valid_state_def]
 ]);
 
 
-val bir_exec_step_valid_state_invar_jmp = prove (
-  ``!p st l. (bir_is_valid_program p /\ bir_is_valid_state p st /\ bir_is_valid_pc p st.bst_pc) ==>
-             bir_is_valid_state p (bir_exec_stmt p (BStmt_Jmp l) st)``,
-SIMP_TAC std_ss [bir_exec_stmt_def, bir_exec_step_valid_state_invar_jmp']);
+val bir_exec_stmtE_valid_state_invar_jmp = prove (
+  ``!p st l. bir_is_valid_state p st ==>
+             bir_is_valid_state p (bir_exec_stmtE p (BStmt_Jmp l) st)``,
+SIMP_TAC std_ss [bir_exec_stmtE_def, bir_exec_stmtE_valid_state_invar_jmp']);
 
 
-val bir_exec_step_valid_state_invar_cjmp = prove (
+val bir_exec_stmtE_valid_state_invar_cjmp = prove (
   ``!p st ex l1 l2.
-       (bir_is_valid_program p /\ bir_is_valid_state p st /\ bir_is_valid_pc p st.bst_pc) ==>
-       bir_is_valid_state p (bir_exec_stmt p (BStmt_CJmp ex l1 l2) st)``,
-SIMP_TAC std_ss [bir_exec_stmt_def, bir_exec_stmt_cjmp_def] >>
+       bir_is_valid_state p st ==>
+       bir_is_valid_state p (bir_exec_stmtE p (BStmt_CJmp ex l1 l2) st)``,
+SIMP_TAC std_ss [bir_exec_stmtE_def, bir_exec_stmt_cjmp_def] >>
 REPEAT STRIP_TAC >>
 Cases_on `bir_dest_bool_val (bir_eval_exp ex st.bst_environ)` >- (
   ASM_SIMP_TAC std_ss [bir_is_valid_state_set_failed]
 ) >>
 rename1 `SOME c` >>
 Cases_on `c` >> (
-  ASM_SIMP_TAC std_ss [bir_exec_step_valid_state_invar_jmp']
+  ASM_SIMP_TAC std_ss [bir_exec_stmtE_valid_state_invar_jmp']
 ));
 
 
-val bir_exec_step_valid_state_invar_halt = prove (
-  ``!p st ex. (bir_is_valid_program p /\ bir_is_valid_state p st /\ bir_is_valid_pc p st.bst_pc) ==>
-               bir_is_valid_state p (bir_exec_stmt p (BStmt_Halt ex) st)``,
+val bir_exec_stmtE_valid_state_invar_halt = prove (
+  ``!p st ex.  bir_is_valid_state p st ==>
+               bir_is_valid_state p (bir_exec_stmtE p (BStmt_Halt ex) st)``,
 
-SIMP_TAC (std_ss++bir_state_ss++bir_status_ss) [bir_exec_stmt_def, bir_exec_stmt_halt_def,
+SIMP_TAC (std_ss++bir_state_ss++bir_status_ss) [bir_exec_stmtE_def, bir_exec_stmt_halt_def,
   bir_is_valid_state_def]);
 
 
-val bir_exec_step_valid_state_invar_assert = prove (
-  ``!p st ex. (bir_is_valid_program p /\ bir_is_valid_state p st /\ bir_is_valid_pc p st.bst_pc) ==>
-               bir_is_valid_state p (bir_exec_stmt p (BStmt_Assert ex) st)``,
 
-SIMP_TAC (std_ss++bir_state_ss++bir_status_ss) [bir_exec_stmt_def, bir_exec_stmt_assert_def] >>
-REPEAT GEN_TAC >> STRIP_TAC >>
-Cases_on `bir_dest_bool_val (bir_eval_exp ex st.bst_environ)` >- (
-  ASM_SIMP_TAC std_ss [bir_is_valid_state_set_failed]
-) >>
-rename1 `SOME c` >>
-Cases_on `c` >| [
-  ASM_SIMP_TAC std_ss [bir_is_valid_state_incr_pc],
-  ASM_SIMP_TAC std_ss [bir_is_valid_state_set_failed]
-]);
+val bir_exec_stmtE_valid_state_invar = store_thm ("bir_exec_stmtE_valid_state_invar",
+``!p st stmt. bir_is_valid_state p st ==>
+              bir_is_valid_state p (bir_exec_stmtE p stmt st)``,
+
+REPEAT STRIP_TAC >>
+Cases_on `stmt` >> (
+  ASM_SIMP_TAC std_ss [
+    bir_exec_stmtE_valid_state_invar_cjmp,
+    bir_exec_stmtE_valid_state_invar_jmp,
+    bir_exec_stmtE_valid_state_invar_halt]
+));
 
 
-val bir_exec_step_valid_state_invar_assume = prove (
-  ``!p st ex. (bir_is_valid_program p /\ bir_is_valid_state p st /\ bir_is_valid_pc p st.bst_pc) ==>
-               bir_is_valid_state p (bir_exec_stmt p (BStmt_Assume ex) st)``,
+val bir_exec_stmtE_env_unchanged = store_thm ("bir_exec_stmtE_env_unchanged",
+``!p st stmt. (bir_exec_stmtE p stmt st).bst_environ = st.bst_environ``,
 
-SIMP_TAC (std_ss++bir_state_ss++bir_status_ss) [bir_exec_stmt_def, bir_exec_stmt_assume_def] >>
-REPEAT GEN_TAC >> STRIP_TAC >>
-Cases_on `bir_dest_bool_val (bir_eval_exp ex st.bst_environ)` >- (
-  ASM_SIMP_TAC std_ss [bir_is_valid_state_set_failed]
-) >>
-rename1 `SOME c` >>
-Cases_on `c` >| [
-  ASM_SIMP_TAC std_ss [bir_is_valid_state_incr_pc],
-  FULL_SIMP_TAC (std_ss++bir_state_ss++bir_status_ss) [bir_is_valid_state_def]
-]);
+REPEAT GEN_TAC >>
+Cases_on `stmt` >> (
+  SIMP_TAC (std_ss++bir_state_ss++bir_status_ss) [
+    bir_exec_stmtE_def, LET_DEF, bir_exec_stmt_cjmp_def,
+    bir_exec_stmt_jmp_def, bir_exec_stmt_halt_def, bir_state_set_failed_def] >>
+  REPEAT CASE_TAC >>
+  FULL_SIMP_TAC (std_ss++bir_state_ss++bir_status_ss) []
+));
+
+
+val bir_exec_stmtE_terminates_no_change = store_thm ("bir_exec_stmtE_terminates_no_change",
+``!p st stmt. ~(bir_state_is_terminated st) ==>
+              (bir_state_is_terminated (bir_exec_stmtE p stmt st)) ==>
+              (((bir_exec_stmtE p stmt st) with bst_status := BST_Running) = st)``,
+
+SIMP_TAC (std_ss++bir_state_ss) [bir_state_is_terminated_def,
+  DB.fetch "-" "bir_state_t_component_equality", bir_exec_stmtB_pc_unchanged] >>
+Cases_on `stmt` >> (
+  SIMP_TAC std_ss [bir_exec_stmtE_def, LET_DEF, bir_exec_stmt_cjmp_def,
+    bir_exec_stmt_jmp_def, bir_exec_stmt_halt_def] >>
+  REPEAT GEN_TAC >> STRIP_TAC >>
+  REPEAT CASE_TAC >>
+  FULL_SIMP_TAC (std_ss++bir_state_ss++bir_status_ss) [bir_state_set_failed_def]
+));
+
+
 
 
 val bir_exec_step_valid_state_invar = store_thm ("bir_exec_step_valid_state_invar",
-``!p st. bir_is_valid_program p /\ bir_is_valid_state p st ==>
+``!p st. bir_is_valid_state p st ==>
          bir_is_valid_state p (bir_exec_step p st)``,
 
 REPEAT STRIP_TAC >>
 IMP_RES_TAC bir_exec_step_valid_THM >>
 Cases_on `bir_state_is_terminated st` >> FULL_SIMP_TAC std_ss [] >>
 Cases_on `stmt` >> (
-  ASM_SIMP_TAC std_ss [bir_exec_step_valid_state_invar_declare,
-    bir_exec_step_valid_state_invar_assign,
-    bir_exec_step_valid_state_invar_cjmp,
-    bir_exec_step_valid_state_invar_jmp,
-    bir_exec_step_valid_state_invar_halt,
-    bir_exec_step_valid_state_invar_assume,
-    bir_exec_step_valid_state_invar_assert]
-));
+  ASM_SIMP_TAC std_ss [bir_exec_stmt_def, bir_exec_stmtE_valid_state_invar, LET_DEF]
+) >>
+rename1 `bir_exec_stmtB stmt st` >>
+Q.ABBREV_TAC `st' = bir_exec_stmtB stmt st` >>
+COND_CASES_TAC >> (
+  ASM_SIMP_TAC std_ss []
+) >>
+`bir_is_valid_state p st'` by METIS_TAC[bir_exec_stmtB_valid_state_invar] >>
+`st'.bst_pc = st.bst_pc` by METIS_TAC[bir_exec_stmtB_pc_unchanged] >>
+FULL_SIMP_TAC (arith_ss++bir_state_ss++bir_pc_ss) [bir_is_valid_state_def,
+  bir_get_current_statement_SOME_B, bir_is_valid_pc_def, bir_pc_next_def] >>
+REPEAT BasicProvers.VAR_EQ_TAC >>
+FULL_SIMP_TAC arith_ss []);
+
 
 
 
 val bir_exec_step_FUNPOW_valid_state_invar = store_thm ("bir_exec_step_FUNPOW_valid_state_invar",
-``!p st n. bir_is_valid_program p /\ bir_is_valid_state p st ==>
+``!p st n. bir_is_valid_state p st ==>
            bir_is_valid_state p (FUNPOW (bir_exec_step p) n st)``,
 
 Induct_on `n` >> (
@@ -1033,28 +823,11 @@ val bir_state_set_failed_SAME_ENV = store_thm ("bir_state_set_failed_SAME_ENV",
   ``!st. (bir_state_set_failed st).bst_environ = st.bst_environ``,
 SIMP_TAC (std_ss++bir_state_ss) [bir_state_set_failed_def]);
 
-
-val bir_state_normalise_pc_SAME_ENV = store_thm ("bir_state_normalise_pc_SAME_ENV",
-  ``!p st. (bir_state_normalise_pc p st).bst_environ = st.bst_environ``,
-REPEAT STRIP_TAC >>
-SIMP_TAC std_ss [bir_state_normalise_pc_def] >>
-CASE_TAC >> SIMP_TAC (std_ss++bir_state_ss) []);
-
-
-val bir_state_incr_pc_SAME_ENV = store_thm ("bir_state_incr_pc_SAME_ENV",
-  ``!p st. (bir_state_incr_pc p st).bst_environ = st.bst_environ``,
-SIMP_TAC (std_ss++bir_state_ss) [bir_state_incr_pc_def, bir_state_normalise_pc_SAME_ENV]);
-
-val bir_state_set_pc_SAME_ENV = store_thm ("bir_state_set_pc_SAME_ENV",
-  ``!p st l. (bir_state_set_pc p st l).bst_environ = st.bst_environ``,
-SIMP_TAC (std_ss++bir_state_ss) [bir_state_set_pc_def, bir_state_normalise_pc_SAME_ENV]);
-
-
 val bir_exec_stmt_jmp_SAME_ENV = store_thm("bir_exec_stmt_jmp_SAME_ENV",
   ``!p st l. (bir_exec_stmt_jmp p l st).bst_environ = st.bst_environ``,
 SIMP_TAC std_ss [bir_exec_stmt_jmp_def] >>
 REPEAT STRIP_TAC >>
-COND_CASES_TAC >> SIMP_TAC (std_ss++bir_state_ss) [bir_state_set_pc_SAME_ENV]);
+COND_CASES_TAC >> SIMP_TAC (std_ss++bir_state_ss) []);
 
 
 val bir_exec_stmt_cjmp_SAME_ENV = store_thm("bir_exec_stmt_cjmp_SAME_ENV",
@@ -1072,25 +845,25 @@ SIMP_TAC (std_ss++bir_state_ss) [bir_exec_stmt_halt_def]);
 
 
 val bir_exec_stmt_assert_SAME_ENV = store_thm("bir_exec_stmt_assert_SAME_ENV",
-  ``!p e st. (bir_exec_stmt_assert p e st).bst_environ = st.bst_environ``,
+  ``!e st. (bir_exec_stmt_assert e st).bst_environ = st.bst_environ``,
 SIMP_TAC (std_ss++bir_state_ss) [bir_exec_stmt_assert_def] >>
 REPEAT STRIP_TAC >>
-REPEAT CASE_TAC >> SIMP_TAC (std_ss++bir_state_ss) [bir_state_incr_pc_SAME_ENV,
+REPEAT CASE_TAC >> SIMP_TAC (std_ss++bir_state_ss) [
    bir_state_set_failed_SAME_ENV]
 );
 
 
 val bir_exec_stmt_assume_SAME_ENV = store_thm("bir_exec_stmt_assume_SAME_ENV",
-  ``!p e st. (bir_exec_stmt_assume p e st).bst_environ = st.bst_environ``,
+  ``!e st. (bir_exec_stmt_assume e st).bst_environ = st.bst_environ``,
 SIMP_TAC (std_ss++bir_state_ss) [bir_exec_stmt_assume_def] >>
 REPEAT STRIP_TAC >>
-REPEAT CASE_TAC >> SIMP_TAC (std_ss++bir_state_ss) [bir_state_incr_pc_SAME_ENV,
+REPEAT CASE_TAC >> SIMP_TAC (std_ss++bir_state_ss) [
    bir_state_set_failed_SAME_ENV]
 );
 
 
 val bir_exec_stmt_declare_ENV = store_thm("bir_exec_stmt_declare_ENV",
-  ``!p vn vty st. (bir_exec_stmt_declare p vn vty st).bst_environ =
+  ``!vn vty st. (bir_exec_stmt_declare vn vty st).bst_environ =
       if (bir_env_varname_is_bound st.bst_environ vn) then st.bst_environ else
       THE (bir_env_update vn (bir_declare_initial_value vty) vty
             st.bst_environ)``,
@@ -1098,7 +871,7 @@ val bir_exec_stmt_declare_ENV = store_thm("bir_exec_stmt_declare_ENV",
 SIMP_TAC (std_ss++bir_state_ss) [bir_exec_stmt_declare_def, LET_DEF] >>
 REPEAT STRIP_TAC >>
 REPEAT CASE_TAC >> (
-   FULL_SIMP_TAC (std_ss++bir_state_ss) [bir_state_incr_pc_SAME_ENV,
+   FULL_SIMP_TAC (std_ss++bir_state_ss) [
      bir_state_set_failed_SAME_ENV]
 ) >>
 Cases_on `st.bst_environ` >> Cases_on `vty` >> (
@@ -1108,8 +881,8 @@ Cases_on `st.bst_environ` >> Cases_on `vty` >> (
 
 
 val bir_exec_stmt_assign_ENV = store_thm("bir_exec_stmt_assign_ENV",
-  ``!p v e st.
-      (bir_exec_stmt_assign p v e st).bst_environ =
+  ``!v e st.
+      (bir_exec_stmt_assign v e st).bst_environ =
       (case bir_env_write v (bir_eval_exp e st.bst_environ) st.bst_environ of
          | SOME env => env
          | NONE => st.bst_environ)``,
@@ -1117,7 +890,7 @@ val bir_exec_stmt_assign_ENV = store_thm("bir_exec_stmt_assign_ENV",
 SIMP_TAC (std_ss++bir_state_ss) [bir_exec_stmt_assign_def, LET_DEF] >>
 REPEAT STRIP_TAC >>
 REPEAT CASE_TAC >> (
-   ASM_SIMP_TAC (std_ss++bir_state_ss) [bir_state_incr_pc_SAME_ENV,
+   ASM_SIMP_TAC (std_ss++bir_state_ss) [
      bir_state_set_failed_SAME_ENV]
 ));
 
@@ -1125,15 +898,21 @@ REPEAT CASE_TAC >> (
 val bir_exec_stmt_ENV_ORDER = store_thm ("bir_exec_stmt_ENV_ORDER",
 ``!p st stmt. bir_env_order st.bst_environ (bir_exec_stmt p stmt st).bst_environ``,
 
+Tactical.REVERSE (Cases_on `stmt`) >- (
+  SIMP_TAC std_ss [bir_exec_stmtE_env_unchanged, bir_exec_stmt_def, bir_env_order_REFL]
+) >>
+rename1 `BStmtB stmt` >>
+SIMP_TAC (std_ss++boolSimps.LIFT_COND_ss++bir_state_ss) [bir_exec_stmt_def, LET_DEF,
+   bir_env_order_REFL] >>
+GEN_TAC >>
+Cases_on `bir_state_is_failed (bir_exec_stmtB stmt st)` >> ASM_REWRITE_TAC[] >>
 Cases_on `stmt` >> (
-  SIMP_TAC (std_ss++boolSimps.LIFT_COND_ss) [bir_exec_stmt_def, bir_exec_stmt_jmp_SAME_ENV,
-    bir_exec_stmt_cjmp_SAME_ENV, bir_exec_stmt_halt_SAME_ENV,
+  SIMP_TAC std_ss [bir_exec_stmtB_def,
     bir_exec_stmt_assert_SAME_ENV, bir_exec_stmt_assume_SAME_ENV,
     bir_env_order_REFL, bir_exec_stmt_assign_ENV,  bir_exec_stmt_declare_ENV]
 ) >- (
-  REPEAT STRIP_TAC >>
   rename1 `bir_var_name v` >>
-  Cases_on `bir_env_varname_is_bound st.bst_environ (bir_var_name v)` >> ASM_REWRITE_TAC[] >>
+  Cases_on `bir_env_varname_is_bound st.bst_environ (bir_var_name v)` >> ASM_REWRITE_TAC[bir_env_order_REFL] >>
   `?env'. bir_env_update (bir_var_name v)
             (bir_declare_initial_value (bir_var_type v)) (bir_var_type v)
             st.bst_environ = SOME env'` by (
