bir_typingScript.sml
@@ -324,18 +324,27 @@ GEN_TAC >> STRIP_TAC >> Induct >> (
 (*  Programs                                                                 *)
 (* ------------------------------------------------------------------------- *)
 
-val bir_is_well_typed_stmt_def = Define `
-  (bir_is_well_typed_stmt (BStmt_Declare _) = T) /\
-  (bir_is_well_typed_stmt (BStmt_Assign v e) = (type_of_bir_exp e = SOME (bir_var_type v))) /\
-  (bir_is_well_typed_stmt (BStmt_Jmp _) = T) /\
-  (bir_is_well_typed_stmt (BStmt_CJmp c _ _) = (type_of_bir_exp c = SOME BoolType)) /\
-  (bir_is_well_typed_stmt (BStmt_Halt e) = (type_of_bir_exp e <> NONE)) /\
-  (bir_is_well_typed_stmt (BStmt_Assert e) = (type_of_bir_exp e = SOME BoolType)) /\
-  (bir_is_well_typed_stmt (BStmt_Assume e) = (type_of_bir_exp e = SOME BoolType))`
+val bir_is_well_typed_stmtE_def = Define `
+  (bir_is_well_typed_stmtE (BStmt_Jmp _) = T) /\
+  (bir_is_well_typed_stmtE (BStmt_CJmp c _ _) = (type_of_bir_exp c = SOME BoolType)) /\
+  (bir_is_well_typed_stmtE (BStmt_Halt e) = (type_of_bir_exp e <> NONE))`
 
+val bir_is_well_typed_stmtB_def = Define `
+  (bir_is_well_typed_stmtB (BStmt_Declare _) = T) /\
+  (bir_is_well_typed_stmtB (BStmt_Assign v e) = (type_of_bir_exp e = SOME (bir_var_type v))) /\
+  (bir_is_well_typed_stmtB (BStmt_Assert e) = (type_of_bir_exp e = SOME BoolType)) /\
+  (bir_is_well_typed_stmtB (BStmt_Assume e) = (type_of_bir_exp e = SOME BoolType))`;
+
+val bir_is_well_typed_stmt_def = Define `
+  (bir_is_well_typed_stmt (BStmtE s) = bir_is_well_typed_stmtE s) /\
+  (bir_is_well_typed_stmt (BStmtB s) = bir_is_well_typed_stmtB s)`;
+
+val bir_is_well_typed_block_def = Define `bir_is_well_typed_block bl <=>
+  ((EVERY bir_is_well_typed_stmtB bl.bb_statements) /\ 
+   (bir_is_well_typed_stmtE bl.bb_last_statement))`;
 
 val bir_is_well_typed_program_def = Define `bir_is_well_typed_program (BirProgram p) <=>
-  (EVERY (\bl. EVERY bir_is_well_typed_stmt bl.bb_statements) p)`;
+  (EVERY bir_is_well_typed_block p)`;
 
 
 val bir_get_current_statement_well_typed = store_thm ("bir_get_current_statement_well_typed",
@@ -345,18 +354,22 @@ val bir_get_current_statement_well_typed = store_thm ("bir_get_current_statement
 
 Cases >> rename1 `BirProgram p` >>
 SIMP_TAC std_ss [bir_is_well_typed_program_def, bir_get_current_statement_def] >>
-REPEAT GEN_TAC >>
+GEN_TAC >>
 Cases_on `(bir_get_program_block_info_by_label (BirProgram p) pc.bpc_label)` >- (
   ASM_SIMP_TAC std_ss []
 ) >>
 rename1 `_ = SOME xy` >> Cases_on `xy` >>
 rename1 `_ = SOME (i, bl)` >>
-ASM_SIMP_TAC std_ss [] >>
-REPEAT STRIP_TAC >>
-`MEM stmt bl.bb_statements` by METIS_TAC[listTheory.MEM_EL] >>
-`MEM bl p` by METIS_TAC [bir_get_program_block_info_by_label_THM, listTheory.MEM_EL] >>
-FULL_SIMP_TAC std_ss [listTheory.EVERY_MEM] >>
-METIS_TAC[]);
+ASM_SIMP_TAC (std_ss++boolSimps.LIFT_COND_ss) [] >>
+Cases_on `EVERY bir_is_well_typed_block p` >> ASM_SIMP_TAC std_ss [] >>
+`bir_is_well_typed_block bl` by (
+  `MEM bl p` by METIS_TAC [bir_get_program_block_info_by_label_THM, listTheory.MEM_EL] >>
+  METIS_TAC[listTheory.EVERY_MEM]
+) >>
+CASE_TAC >> (
+  FULL_SIMP_TAC std_ss [bir_is_well_typed_block_def, bir_is_well_typed_stmt_def]
+) >>
+METIS_TAC[listTheory.EVERY_MEM, listTheory.MEM_EL]);
 
 
 val _ = export_theory();
